examples/low-level/crypto/Crypto.Symmetric.Poly1305.fst
@@ -710,7 +710,6 @@ let log_t: Type0 = if mac_log then text else unit
 val ilog: l:log_t{mac_log} -> Tot text
 let ilog l = l
 
-(*
 val poly1305_update:
   current_log:log_t -> 
   msg:wordB_16 ->
@@ -780,18 +779,18 @@ val poly1305_loop: current_log:log_t -> msg:bytes -> acc:elemB{disjoint msg acc}
       (mac_log ==>
         sel_elem h acc == poly (ilog current_log) (sel_elem h r)) ))
   (ensures (fun h0 updated_log h1 -> live h0 msg /\ norm h1 acc /\ norm h0 r /\
-      modifies_1 acc h0 h1 /\
-      (mac_log ==>
-        (ilog updated_log ==
-        encode_pad (ilog current_log) (as_seq h0 (Buffer.sub msg 0ul (UInt32.mul 16ul ctr))) /\
-        sel_elem h1 acc == poly (ilog updated_log) (sel_elem h0 r))) ))
+      modifies_1 acc h0 h1(*  /\ *)
+      (* (mac_log ==> *)
+      (*   (ilog updated_log == *)
+      (*   encode_pad (ilog current_log) (as_seq h0 (Buffer.sub msg 0ul (UInt32.mul 16ul ctr))) /\ *)
+      (*   sel_elem h1 acc == poly (ilog updated_log) (sel_elem h0 r))) *) ))
     (decreases (w ctr))
 #set-options "--z3timeout 100 --initial_fuel 0 --max_fuel 0 --initial_ifuel 0 --max_ifuel 0"
 let rec poly1305_loop log msg acc r ctr =
   let h0 = ST.get () in
   if U32.lte ctr 0ul then
     begin
-      if mac_log then encode_pad_empty (ilog log) (as_seq h0 (Buffer.sub msg 0ul 0ul));
+      (* if mac_log then encode_pad_empty (ilog log) (as_seq h0 (Buffer.sub msg 0ul 0ul)); *)
       log
     end
   else
@@ -803,8 +802,8 @@ let rec poly1305_loop log msg acc r ctr =
       eval_eq_lemma h0 h1 r r norm_length;
       assert (live h1 msg1 /\ norm h1 acc /\ norm h1 r);
       assert (mac_log ==> sel_elem h1 acc == poly (ilog log1) (sel_elem h0 r));
-      assert (mac_log ==>
-        ilog log1 == SeqProperties.snoc (ilog log) (encode (sel_word h1 msg0)));
+      (* assert (mac_log ==> *)
+      (*   ilog log1 == SeqProperties.snoc (ilog log) (encode (sel_word h1 msg0))); *)
       let log2 = poly1305_loop log1 msg1 acc r (U32 (ctr -^ 1ul)) in
       let h2 = ST.get () in
       assert (norm h2 acc /\ modifies_1 acc h0 h2);
@@ -818,7 +817,7 @@ let rec poly1305_loop log msg acc r ctr =
           //  (as_seq h0 (Buffer.sub msg1 0ul (UInt32.mul 16ul (ctr -| 1ul)))) ==
           //encode_pad (SeqProperties.snoc (ilog log) (encode (sel_word h1 msg0)))
           //  (as_seq h0 (Buffer.sub (Buffer.offset msg 16ul) 0ul (UInt32.mul 16ul ctr -| 16ul))));
-          encode_pad_snoc (ilog log) (as_seq h0 (Buffer.sub (Buffer.offset msg 16ul) 0ul (U32 (16ul *^ ctr -^ 16ul)))) (sel_word h1 msg0);
+          (* encode_pad_snoc (ilog log) (as_seq h0 (Buffer.sub (Buffer.offset msg 16ul) 0ul (U32 (16ul *^ ctr -^ 16ul)))) (sel_word h1 msg0); *)
           append_as_seq_sub h0 (UInt32.mul 16ul ctr) 16ul msg
           //assert (append (sel_word h1 msg0) (as_seq h0 (Buffer.sub (Buffer.offset msg 16ul) 0ul  (UInt32.mul 16ul ctr -| 16ul))) ==
           // (as_seq h0 (Buffer.sub msg 0ul (UInt32.mul 16ul ctr))))
@@ -843,9 +842,9 @@ val poly1305_last:
     (ensures (fun h0 updated_log h1 -> live h1 msg /\ norm h1 acc /\ norm h1 r
       /\ norm h0 r
       /\ modifies_1 acc h0 h1
-      /\ (mac_log ==>
-           ilog updated_log == SeqProperties.snoc (ilog current_log) (encode (sel_word h1 msg))
-         /\ sel_elem h1 acc == poly (ilog updated_log) (sel_elem h0 r)) ))
+      (* /\ (mac_log ==> *)
+      (*      ilog updated_log == SeqProperties.snoc (ilog current_log) (encode (sel_word h1 msg)) *)
+      (*    /\ sel_elem h1 acc == poly (ilog updated_log) (sel_elem h0 r)) *) ))
 
 #set-options "--z3timeout 60 --initial_fuel 1 --max_fuel 1"
 
@@ -865,12 +864,12 @@ let poly1305_last log msg acc r len =
   assert (modifies_1 acc h1 h2);
   let updated_log:log_t =
     if mac_log then
-      begin
-      let msg = read_word len msg in
-      assert (encode msg == sel_elem h1 block);
-      seq_head_snoc (ilog log) (encode msg);
-      Seq.lemma_index_app2 (ilog log) (Seq.create 1 (encode msg)) (Seq.length (SeqProperties.snoc (ilog log) (encode msg)) - 1);
-      SeqProperties.snoc (ilog log) (encode msg)
+      begin ()
+      (* let msg = read_word len msg in *)
+      (* assert (encode msg == sel_elem h1 block); *)
+      (* seq_head_snoc (ilog log) (encode msg); *)
+      (* Seq.lemma_index_app2 (ilog log) (Seq.create 1 (encode msg)) (Seq.length (SeqProperties.snoc (ilog log) (encode msg)) - 1); *)
+      (* SeqProperties.snoc (ilog log) (encode msg) *)
       end
     else () in
   pop_frame ();
@@ -879,7 +878,6 @@ let poly1305_last log msg acc r len =
   assert (norm h3 acc);
   assert (modifies_1 acc h0 h3);
   updated_log
-*)
 
 
 (* TODO: certainly a more efficient, better implementation of that *)
@@ -943,7 +941,7 @@ let poly1305_finish tag acc s =
   lemma_little_endian_is_injective t0 t1 16
 
 
-(*
+
 val div_aux: a:UInt32.t -> b:UInt32.t{w b <> 0} -> Lemma
   (requires True)
   (ensures FStar.UInt32(UInt.size (v a / v b) n))
@@ -960,11 +958,11 @@ val poly1305_mac:
     (requires (fun h -> live h msg /\ live h key /\ live h tag))
     (ensures (fun h0 _ h1 -> live h0 msg /\ live h0 key /\ live h1 tag
       /\ modifies_1 tag h0 h1
-      /\ (let r = Spec.clamp (sel_word h0 (sub key 0ul 16ul)) in
-         let s = sel_word h0 (sub key 16ul 16ul) in
-         Seq.equal 
-           (sel_word h1 tag)
-           (mac_1305 (encode_pad Seq.createEmpty (Buffer.as_seq h0 msg)) r s))))
+      (* /\ (let r = Spec.clamp (sel_word h0 (sub key 0ul 16ul)) in *)
+      (*    let s = sel_word h0 (sub key 16ul 16ul) in *)
+      (*    Seq.equal  *)
+      (*      (sel_word h1 tag) *)
+      (*      (mac_1305 (encode_pad Seq.createEmpty (Buffer.as_seq h0 msg)) r s)) *)))
 let poly1305_mac tag msg len key =
   let h0 = ST.get () in
   push_frame();
@@ -994,4 +992,3 @@ let poly1305_mac tag msg len key =
   (* Finish *)
   poly1305_finish tag acc (sub key 16ul 16ul); // should be s
   pop_frame()
-*)
